Strata/Languages/Core/DDMTransform/Translate.lean
@@ -1187,6 +1187,23 @@ partial def translateStmt (p : Program) (bindings : TransBindings) (arg : Arg) :
     -- Add the function to boundVars for subsequent statements.
     let updatedBindings := { bindings with boundVars := bindings.boundVars.push funcBinding }
     return ([.funcDecl decl md], updatedBindings)
+  | q`Core.typeDecl_statement, #[namea, argsa] =>
+    let name ← translateIdent String namea
+    let numargs ← match argsa with
+      | .option _ (.some binds) => do
+        let args ← translateMonoDeclList bindings binds
+        pure args.length
+      | .option _ .none => pure 0
+      | _ => TransM.error s!"Invalid type arguments {repr argsa}"
+    let md ← getOpMetaData op
+    -- Add the type to the type context for subsequent statements
+    let typeArgs := List.replicate numargs "_ty"
+    let ids := typeArgs.mapIdx (fun i elem => (elem ++ toString i))
+    let typeBinding : LExpr Core.CoreLParams.mono := .op () name none
+    let updatedBindings := { bindings with 
+      boundVars := bindings.boundVars.push typeBinding,
+      boundTypeVars := bindings.boundTypeVars ++ ids.toArray }
+    return ([.typeDecl name numargs md], updatedBindings)
   | name, args => TransM.error s!"Unexpected statement {name.fullName} with {args.size} arguments."
 
 partial def translateBlock (p : Program) (bindings : TransBindings) (arg : Arg) :
